src/LocalReasoning.v
@@ -2,7 +2,7 @@
 (* Clément Blaudeau - Lamp@EPFL 2021 *)
 (** This file defines the main result of local reasoning, built upon wellformedness, compatibility, scopability and stackability. In a wellformed, fully initialized context, a newly created object can only access hot (transitively fully initialized) locations. *)
 
-From Celsius Require Export Trees Eval PartialMonotonicity Reachability Compatibility Scopability Stackability Wellformedness.
+From Celsius Require Export Scopability Compatibility PartialMonotonicity Stackability.
 Require Import ssreflect ssrbool Psatz Sets.Ensembles List.
 Import ListNotations.
 Open Scope nat_scope.
@@ -34,17 +34,17 @@ Qed.
 
 (* Then the main theorem : *)
 Theorem Local_reasoning:
-  forall e σ σ' ρ ψ l k,
-    ⟦e⟧(σ, ρ, ψ)(k) = (Success l σ') ->
+  forall e σ ρ ψ v σ',
+    ⟦e⟧p(σ, ρ, ψ) --> (v, σ') ->
     wf σ ->
     (codom ρ ∪ {ψ}) ⪽ σ ->
     (σ ⊫ ((codom ρ) ∪ {ψ}) : hot) ->
-    σ' ⊨ l : hot.
+    σ' ⊨ v : hot.
 Proof.
   intros.
-  assert (σ' ⊫ (Singleton Loc l) : hot). {
+  assert (σ' ⊫ (Singleton Loc v) : hot). {
     eapply local_reasoning;
-      eauto using stackability_theorem with pM stk cmpt wf lia.
+      eauto using stk_theorem with pM stk cmpt wf lia.
     eapply scopability_theorem in H; eauto with pM wf lia; steps. }
   eapply H3; eauto using In_singleton.
 Qed.
