src/Scopability.v
@@ -4,7 +4,7 @@
 The main idea is pretty natural: to ensure that newly created objects are hot, we need to check that, transitively, all locations reachable from the attributes of the object are intialized. To do so, we need to be able to reason about the set of locations that are reachable from a set of attributes in a given store. Given two stores [σ] and [σ'], and two sets of locations [L] and [L'], the pair [(σ, L)] "scopes" [(σ',L')] if all locations reachable from [L'] in [σ'] were already reachable from [L] in [σ].
  But as we allow to manipulate objects under initialization, we also need to consider a notion of "preservation" : scoping relations that are maintained when updating from one store to another. *)
 
-From Celsius Require Export PartialMonotonicity Compatibility Wellformedness Reachability.
+From Celsius Require Export PartialMonotonicity Compatibility Wellformedness Reachability Tactics.
 Require Import ssreflect ssrbool Psatz Sets.Ensembles List.
 Import ListNotations.
 Open Scope nat_scope.
@@ -15,7 +15,14 @@ Definition scoping (σ σ': Store) (L L': Ensemble Loc) :=
   L ⪽ σ ->
   L' ⪽ σ' ->
   (forall l, l < (dom σ) -> (σ' ⊫ L' ⇝ l) -> σ ⊫ L ⇝ l).
-Notation "a ⋖ b" := (scoping (fst a) (fst b) (snd a) (snd b)) (at level 81).
+
+Notation "( σ1 , L1 )  ⋖  ( σ2 , L2 )" := (scoping σ1 σ2 L1 L2) (at level 0).
+Notation "( σ1 , { l } )  ⋖  ( σ2 , L2 )" := (scoping σ1 σ2 {l} L2) (at level 0).
+Notation "( σ1 , L1 )  ⋖  ( σ2 , { l } )" := (scoping σ1 σ2 L1 {l}) (at level 0).
+Notation "( σ1 , { l1 } )  ⋖  ( σ2 , { l2 } )" := (scoping σ1 σ2 {l1} {l2}) (at level 0).
+
+
+(* Notation "a ⋖ b" := (scoping (fst a) (fst b) (snd a) (snd b)) (at level 81).*)
 
 (* The scoping preservation, with technical choices of hypothesis: *)
 Definition scoping_preservation (σ1 σ2: Store) (L: LocSet) :=
@@ -32,6 +39,7 @@ Notation "σ1 ⇝ σ2 ⋖ L" := (scoping_preservation σ1 σ2 L) (at level 81, �
 
 Global Hint Unfold scoping : scoping.
 Global Hint Unfold scoping_preservation : scoping.
+Global Hint Unfold reachability_set: scoping.
 Global Hint Resolve Union_introl: scoping.
 Global Hint Resolve Union_intror: scoping.
 
@@ -59,11 +67,8 @@ Lemma scoping_subset :
     (σ1, L1) ⋖ (σ2, L2∪L) ->
     L2∪L ⪽ σ2 ->
     (σ1, L1) ⋖ (σ2, L).
-Proof.
-  unfold scoping, reachability_set; steps; eauto.
-  eapply H => //.
-  exists l'; steps; eauto with scoping.
-  apply Union_intror; steps.
+Proof with (eauto with scoping).
+  unfold scoping, reachability_set; steps ...
 Qed.
 Global Hint Resolve scoping_subset: scoping.
 
@@ -84,9 +89,8 @@ Lemma scoping_union_introl :
     (σ1, L) ⋖ (σ2, L1∪L2) ->
     (σ1, L) ⋖ (σ2, L1).
 Proof.
-  unfold scoping, reachability_set; simpl; steps.
-  eapply_any; eauto.
-  eexists; eauto with scoping.
+  unfold scoping, reachability_set; steps.
+  eauto with scoping.
 Qed.
 Global Hint Resolve scoping_union_introl: scoping.
 
@@ -96,9 +100,8 @@ Lemma scoping_union_intror :
     (σ1, L)  ⋖ (σ2, L1∪L2) ->
     (σ1, L)  ⋖ (σ2, L2).
 Proof.
-  unfold scoping, reachability_set; simpl; steps.
-  eapply_any; eauto.
-  eexists; eauto with scoping.
+  unfold scoping, reachability_set; steps.
+  eauto with scoping.
 Qed.
 Global Hint Resolve scoping_union_intror: scoping.
 
@@ -109,6 +112,7 @@ Lemma scoping_reachability:
     (σ, {l1}) ⋖ (σ, {l2}).
 Proof.
   unfold scoping, reachability_set ; steps.
+  eauto with scoping.
   exists l1; try inSingleton; steps; eauto with scoping rch.
 Qed.
 Global Hint Resolve scoping_reachability: scoping.
@@ -134,11 +138,11 @@ Lemma preserving_transitivity:
     (σ1, L1) ⋖ (σ2, L2) ->
     dom σ1 <= dom σ2 ->
     σ1 ⇝ σ3 ⋖ L1.
-Proof.
-  unfold scoping_preservation ; light; destructs.
-  split; [eapply_any |]; light.
-  eapply H4; eauto with wf lia.
-  eapply scoping_transitivity with σ1 L1; eauto with wf lia rch.
+Proof with (eauto with wf lia).
+  unfold scoping_preservation ; light.
+  split; [eapply_any |]; steps.
+  eapply_any ...
+  eapply scoping_transitivity with σ1 L1 ...
 Qed.
 Global Hint Resolve preserving_transitivity: scoping.
 
@@ -210,13 +214,14 @@ Lemma scopability_add_env:
       (σ0, L0) ⋖ ([I ↦ (c, e0 ++ [v])] (s), L2).
 Proof.
   intros; unfold scoping; simpl; intros.
-  destruct H8; destructs.
+  destruct H8; steps.
   assert (s ⊨ x ⇝ l \/ ((s ⊨ x ⇝ I) /\ (s ⊨ v ⇝ l))) by
       eauto using reachability_add_env with updates.
   steps;
     [ eapply H4 | eapply H3] ;
     simpl; try (eexists; split); eauto with wf.
 Qed.
+Hint Resolve scopability_add_env: scoping.
 
 
 (** ** Assignment results *)
@@ -232,7 +237,7 @@ Lemma scopability_assignment:
     σ2' = [l ↦ (C, ω')]σ2 ->
     (σ1 ⇝ σ2' ⋖ L1) /\ ((σ1, L1) ⋖ (σ2', {l})).
 Proof.
-  unfold scoping_preservation; light; destructs.
+  unfold scoping_preservation; light; flatten.
   split.
   - (* σ1 ⇝ σ2' ⋖ L1 *)
     split; eauto.
@@ -242,7 +247,7 @@ Proof.
     intros.
     assert ((σ0, L0) ⋖ (σ2, L)) as B1 by eauto.
     assert ((σ0, L0) ⋖ (σ2, {l'})) as C1 by eauto using scoping_transitivity.
-    destruct H7; destructs.
+    destruct H7; steps.
     eapply storeSubset_update in H5.
     destruct_eq (l = l'); subst.
     + (* l = l' , the assignment is weakening *)
@@ -250,18 +255,18 @@ Proof.
     + (* l ≠ l' *)
       pose proof (reachability_dom _ _ _ H9).
       (* Key case analysis : is the modified value in the path ? *)
-      eapply reachable_path_reachability in H9; light; destructs; subst; update_dom.
+      eapply reachable_path_reachability in H9; light; flatten; subst; update_dom.
       * eapply B1; (try exists l0); simpl; eauto with rch.
-      * pose proof H10.
-        eapply reachable_path_assignment in H10 as [Hedge | Hpath]; eauto.
-        ** eapply contains_edge_last_edge in Hedge; destructs.
+      * pose proof H7.
+        eapply reachable_path_assignment in H7 as [Hedge | Hpath]; eauto.
+        ** eapply contains_edge_last_edge in Hedge; flatten.
            assert (σ2 ⊨ l' ⇝ l0). {
              eapply reachable_path_reachability.
-             eapply contains_edge_split in Hedge0 ; destructs; eauto.
+             eapply contains_edge_split in Hedge0 ; flatten; eauto.
              rewrite Hedge2 in H9.
              eapply (reachable_path_app2 _ l' (l::p2) (l0::p1')) in H9.
              eapply reachable_path_assignment in H9; eauto.
-             destructs; eauto with rch.
+             flatten; eauto with rch.
              exfalso; apply Hedge1.
              eapply contains_edge_last; eauto. }
            eapply C1; simpl; eauto with wf rch.
@@ -279,7 +284,7 @@ Proof.
     + (* if l = l', the assignment is weakening *)
       eapply H0; try (eexists; split);
         eauto using In_singleton, reachability_weaken_assignment with wf rch updates.
-    + eapply reachable_path_reachability in H9; light; destructs; subst; update_dom.
+    + eapply reachable_path_reachability in H9; light; flatten; subst; update_dom.
       * eapply H0; try (eexists; split);
           eauto using In_singleton, reachability_weaken_assignment with wf rch updates.
       * pose proof H.
@@ -288,17 +293,17 @@ Proof.
         ++ assert (l' < dom σ2). {
              erewrite <- update_dom.
              eapply reachability_dom2, reachable_path_is_reachable; eauto with rch.
-             unfold contains_edge in Hedge; destructs.
+             unfold contains_edge in Hedge; flatten.
              rewrite Hedge; apply in_app_iff; steps. }
            eapply H1; try (eexists; split); eauto using In_singleton with rch wf.
-           eapply_anywhere contains_edge_last_edge; destructs.
+           eapply_anywhere contains_edge_last_edge; flatten.
            eapply reachable_path_reachability.
            destruct_eq (l' = l0); subst ; [left; split; eauto; lia | right ].
-           eapply contains_edge_split in Hedge0 ; destructs; [steps | eauto].
+           eapply contains_edge_split in Hedge0 ; flatten; [steps | eauto].
            rewrite Hedge2 in H7.
            eapply (reachable_path_app2 _ l' (l::p2) (l0::p1')) in H7.
            eapply reachable_path_assignment in H7; eauto.
-           destructs; eauto with rch.
+           flatten; eauto with rch.
            exfalso; apply Hedge1.
            eapply contains_edge_last; eauto.
         ++ eapply H0; try (eexists; split);
@@ -307,198 +312,117 @@ Proof.
 Qed.
 
 (** ** Evaluation-maintained results *)
-(** We start by defining the scopability property we want the evaluator to maintain. *)
-Definition scopability_prop n :=
-  forall e σ σ' ρ ψ l,
-    ⟦e⟧(σ, ρ, ψ)(n) = (Success l σ') ->
-    wf σ -> (codom ρ) ∪ {ψ} ⪽ σ ->
-    ((σ, ((codom ρ) ∪ {ψ})) ⋖ (σ', {l})) /\ (σ ⇝ σ' ⋖ ((codom ρ) ∪ {ψ})) .
-
-(* We show the induction case for lists *)
-Lemma scopability_list_aux:
-  forall n,
-    (forall k, k < S n -> scopability_prop k) (**r strong induction hypothesis *) ->
-    forall el σ ρ ψ  ρ' σ' ,
-      (⟦_ el _⟧ (σ, ρ, ψ )(n)) = Success_l ρ' σ' ->
-      wf σ ->
-      (codom ρ ∪ {ψ}) ⪽ σ ->
-      ((σ, codom ρ ∪ {ψ}) ⋖ (σ', codom ρ')) /\ (σ ⇝ σ' ⋖ codom ρ ∪ {ψ}).
-Proof.
-  unfold scopability_prop; intros.
-  destruct n; try discriminate.
-  simpl in * |- .
-  (* We generalize the induction hypothesis *)
-  assert (forall el ρ' σ1 σ2 acc,
-             fold_left (eval_list_aux ρ ψ n) el (Success_l acc σ1) = Success_l ρ' σ2 ->
-             wf σ1 ->
-             dom σ <= dom σ1 ->
-             σ ⇝ σ1 ⋖ (codom ρ ∪ {ψ}) ->
-             (codom acc) ⪽ σ1 ->
-             ((σ, codom ρ ∪ {ψ}) ⋖ (σ1, codom acc)) ->
-             ((σ, codom ρ ∪ {ψ}) ⋖ (σ2, codom ρ')) /\
-             (σ ⇝ σ2 ⋖ codom ρ ∪ {ψ}) /\
-             codom ρ' ⪽ σ2) as H_ind. {
-    induction el0; [solve [steps] |].
-    intros L σ1 σ2 acc Hfold; intros.
-    destruct n; simpl in Hfold; [rewrite_anywhere foldLeft_constant => // |].
-    destruct_eval_with_name Heval.
-    repeat eval_dom || eval_wf.
-    eapply H in Heval; try lia; try destructs; eauto with wf.
-    eapply IHel0 in Hfold; try rewrite codom_cons; eauto with scoping; try lia.
-    + eauto with wf.
-    + eapply scoping_union.
-      ++ apply scoping_transitivity with σ1 (codom ρ ∪ {ψ});
-           eauto with wf scoping.
-      ++ apply Heval1; eauto with lia scoping.
-  }
-  eapply H_ind in H0; try erewrite codom_empty_union; steps; eauto with wf scoping.
-  apply scoping_reflexivity.
-  intros l'; steps. inversion H3.
-Qed.
-
-(** Then the induction case for initialization of a new object *)
-Lemma scopability_init_aux:
-  forall n,
-    (forall k, k < S n -> scopability_prop k) (**r strong induction hypothesis *) ->
-    forall σ L L1 I fields σ1 σ2,
-      fold_left (init_field L1 I n) fields (Some σ1) = Some σ2 ->
-      dom σ <= dom σ1 ->
-      I < dom σ1 ->
-      wf σ1 ->
-      (codom L1 ∪ {I}) ⪽ σ1 ->
-      ((σ, L) ⋖ (σ1, (codom L1) ∪ {I})) ->
-      (σ ⇝ σ1 ⋖ L) ->
-
-      ((σ, L) ⋖ (σ2, (codom L1) ∪ {I})) /\ (σ ⇝ σ2 ⋖ L) /\ (dom σ1 <= dom σ2).
-Proof.
-  unfold scopability_prop. intros n H_strong σ L L1 I.
-  induction fields; [steps |]; intros; simpl in H.
-  destruct n; [rewrite_anywhere foldLeft_constant => // |]; simpl in H.
-  destruct a as [_ e]; destruct_eval.
-  rewrite {2}/assign_new in H.
-  destruct (getObj s I) eqn:G; try solve [rewrite_anywhere  foldLeft_constant => //].
-  destruct o.
-  eval_dom; eval_wf.
-  eapply H_strong in H6; eauto with wf; destructs.
-  eapply IHfields in H; eauto;
-    destructs; repeat split;
-      try update_dom; try lia;
-        try solve [eapply_any; eauto];
-        eauto with wf pM.
-  ++ unfold wf; intros; update_dom.
-     getObj_update; destructs; try invert_constructor_equalities; subst; eauto.
-     eapply_anywhere getVal_add; destructs; eauto with wf updates.
-  ++ eapply storeSubset_trans with s; update_dom; eauto with wf lia.
-  ++ eapply scoping_transitivity with σ1 _; try solve [eapply_any]; eauto with scoping.
-     apply scopability_add_env; eauto with wf lia.
-     eapply_any; eauto with scoping.
-  ++ intros.
-     eapply preserving_transitivity; eauto.
-     eapply preserving_transitivity; eauto.
-     unfold scoping_preservation; split; intros; eauto using scopability_add_env with wf.
-     update_dom; lia.
-Qed.
-
+Hint Extern 1 => repeat rch_singleton: scoping.
+Hint Extern 1 => rewrite update_dom : updates.
 
 (** ** Main Scopability theorem *)
 (** We show the main theorem. As for wellformedness theorem, we have to make a custom proof. We use the results shown for initialization, lists and assignment *)
 Theorem scopability_theorem:
-  forall n, scopability_prop n.
-Proof.
-  apply strong_induction.
-  intros n H_strong. unfold scopability_prop; intros.
-  destruct n => //.
-  destruct e as [x | this | e0 f | e0 m el | C el | e0 f e1 e2];
-    simpl in H; repeat destruct_match;
-      try discriminate;
-      try (destruct n ; [discriminate |]);
-      try invert_constructor_equalities; subst.
-  + (* e = x *)
-    unfold scoping; steps; try rch_singleton; eauto with scoping.
-    eexists; split; eauto.
-    eapply Union_introl, nth_error_In; eauto.
-  + (* e = this *)
-    unfold scoping; steps; try rch_singleton; eauto with scoping.
-    eexists; eauto using Union_intror, In_singleton.
-  + (* e = e0.f *)
-    unfold scoping; intros; simpl.
-    eval_dom; eval_wf.
-    eapply H_strong in matched; try lia.
-    intuition auto.
-    assert ((σ', {v}) ⋖ (σ', {l})) as B1 by eauto with rch scoping updates.
-    assert ((σ,  (codom ρ) ∪ ({ψ})) ⋖ (σ', {l})) as C1 by
-          (eapply scoping_transitivity with σ' {v}; eauto with updates rch wf); steps.
-  + (* e = e0.m(l0) *)
-    rename s into σ0, l0 into ρ', v into l0, e into ω, matched0 into A5,
-    s0 into σ_n, body into e_m, l into l_m, σ' into σ_m. (* Renaming for readability *)
-    repeat eval_dom || eval_wf. (* We extract the wellformedness results of successful evaluations *)
-    eapply H_strong in H, matched; try lia. (* We apply the induction hypothesis on sub evaluations *)
-    eapply scopability_list_aux in matched6;
-      try lia; eauto with wf ; destructs. (* We use the list induction case proven before *)
-    assert ((codom ρ' ∪ {l0}) ⪽ σ_n) by eauto with wf.
-    repeat destructs || modus_ponens.
-    nat_le_trans.
-    assert ((σ, (codom ρ) ∪ {ψ}) ⋖ (σ0, (codom ρ) ∪ {ψ})) as A4 by eauto with scoping wf pM.
-    assert ((σ, codom ρ ∪ {ψ}) ⋖ (σ_n, (codom ρ') ∪ {l0}) ) as A6. {
-      apply scoping_union.
-       ++ eapply scoping_transitivity with σ0 _; eauto; eauto with wf lia.
-       ++ eapply matched1; eauto with wf lia.
-    }
-    split; eauto with scoping.
-  + (* e = new C(l0) *)
-    rename matched into C0, s into σ_n, l0 into L.
-    assert (dom σ <= dom σ_n) by eauto with pM.
-    eval_wf.
-    eapply scopability_list_aux in C0; eauto with wf; destructs.
-    simpl in matched0. repeat (destruct_match; try discriminate).
-    assert (dom (σ_n ++ [(C, [])]) = S (dom σ_n)) as H_dom
-        by (unfold dom; rewrite app_length; simpl; lia).
-    eapply scopability_init_aux with (σ := σ) (L := codom ρ ∪ {ψ}) in matched0;
-      try rewrite H_dom; eauto with wf lia.
-    ++ destructs; split => //.
+  forall e σ ρ ψ v σ',
+    ⟦e⟧p (σ, ρ, ψ) --> (v, σ') ->
+    (codom ρ) ∪ {ψ} ⪽ σ -> wf σ ->
+    ((σ, ((codom ρ) ∪ {ψ})) ⋖ (σ', {v})) /\ (σ ⇝ σ' ⋖ ((codom ρ) ∪ {ψ})) .
+Proof with (timeout 10 eauto with scoping wf rch lia).
+  intros.
+  move: H0 H1.
+  induction H using evalP_ind2 with
+    (Pl := fun _ σ ρ ψ vl σ' _ =>
+             (codom ρ ∪ {ψ}) ⪽ σ ->
+             wf σ ->
+             ((σ, codom ρ ∪ {ψ}) ⋖ (σ', codom vl)) /\ (σ ⇝ σ' ⋖ codom ρ ∪ {ψ}))
+    (Pin := fun _ ψ ρ σ σ' _   => forall L σ0,
+                dom σ0 <= dom σ ->
+                (codom ρ ∪ {ψ}) ⪽ σ ->
+                ((σ0, L) ⋖ (σ, (codom ρ) ∪ {ψ})) ->
+                (σ0 ⇝ σ ⋖ L) ->
+                wf σ ->
+                ((σ0, L) ⋖ (σ', (codom ρ) ∪ {ψ})) /\ (σ0 ⇝ σ' ⋖ L));
+    unfold assign, assign_new in * ; intros; eval_dom; eval_wf;
+    try solve [rch_singleton; eauto with scoping lia].
+  - (* e = x *)
+    unfold scoping; steps...
+    exists l ...
+  - (* e = e0.f *)
+    unfold scoping; steps; rch_singleton ...
+    assert ((σ,  (codom ρ) ∪ ({ψ})) ⋖ (σ1, {l})) as C1 by
+        (eapply scoping_transitivity with σ1 {l1}; eauto with updates rch wf scoping).
+    eapply C1 ; steps ...
+  - (* e = e0.m(l0) *)
+    destruct IHevalP1, IHevalP2; eauto with wf.
+    destruct IHevalP3; eauto with wf.
+    assert ((σ, (codom ρ) ∪ {ψ}) ⋖ (σ1, (codom ρ) ∪ {ψ})) as A4 by eauto with scoping wf pM.
+    assert ((σ, codom ρ ∪ {ψ}) ⋖ (σ2, (codom vl2) ∪ {v1}) ) as A6 by
+        (eapply scoping_union; eauto with scoping wf pM lia).
+    split.
+    + eapply scoping_transitivity with σ2 ( codom vl2 ∪ {v1}) ...
+    + eapply preserving_transitivity with σ2 ( codom vl2 ∪ {v1}) ...
+  - (* e = new C(l0) *)
+    destruct IHevalP; eauto with wf.
+    specialize IHevalP0 with (codom ρ ∪ {ψ}) σ.
+    assert (dom σ1 <= dom (σ1 ++ [(C, [])])) by (rewrite dom_app; lia).
+    assert (Heq:length σ1 = dom σ1) by steps. rewrite Heq in IHevalP0, H__init |- *.
+    destruct IHevalP0; eauto with wf .
+    + rewrite dom_app. steps.
+    + eapply storeSubset_union ...
+      eapply storeSubset_singleton3 .
+      rewrite dom_app /dom ... (* storeSubset_add_empty ? *)
+    + intros ? ; steps.
+      move : H9 => [l0 [H__l0 H__rch]].
+      inversion H__l0; steps.
+      * eapply H3 ...
+        eapply reachability_empty with (C := C) ...
+      * inSingleton.
+        eapply reachability_not_empty in H__rch ...
+    + eapply preserving_transitivity; eauto.
+      unfold scoping_preservation; steps; eauto.
+      unfold scoping; steps.
+      eapply reachability_empty in H15 ...
+    + flatten; split => //.
        eapply scoping_union_intror ; eauto with wf scoping.
-       fold (dom σ_n) in *. rewrite H_dom in matched3.
-       apply storeSubset_union; eauto with wf lia.
-       eapply storeSubset_trans with σ_n; eauto; lia.
-    ++ eapply storeSubset_union.
-       +++ eapply storeSubset_trans with σ_n ; eauto with wf lia.
-       +++ eapply storeSubset_singleton3; unfold dom in * ; eauto with wf lia.
-    ++ intros x ; steps.
-       eapply_anywhere reachability_empty;
-         unfold dom in * ; [| eauto using PeanoNat.Nat.lt_le_trans ].
-       eapply C1; steps.
-       inversion H4; steps. eexists.
-       inversion H6; try inSingleton; steps; eauto.
-       eapply reachability_dom2 in H7; exfalso; unfold dom in *; lia.
-    ++ eapply preserving_transitivity; eauto.
-       unfold scoping_preservation; split; intros; eauto.
-       unfold scoping; simpl; intros.
-       assert (reachability_set σ_n L1 l) by eauto using PeanoNat.Nat.lt_le_trans, reachability_empty.
-       steps.
-  + (* e = e0.f = e1; e2 *)
-    rename matched into A0, s into σ0, v into l0, s0 into σ1, v0 into l1, matched0 into B0.
-    repeat eval_dom || eval_wf.
-    unfold assign in *;
-      repeat destruct_match; try solve [eapply nth_error_None in matched; unfold dom in *; lia].
-    update_dom.
-    assert (wf [l0 ↦ (c, [f ↦ l1] (e))] (σ1)) by eauto with wf.
-    eval_wf; [eapply storeSubset_trans with σ; update_dom; eauto with lia |].
-    eapply H_strong in A0, B0, H; try lia; eauto; repeat modus_ponens || destructs.
-    destruct H; eauto with wf.
-    unfold assign in *.
-    destruct H6; [eapply storeSubset_trans with σ1; update_dom; eauto with wf lia |].
-    epose proof (scopability_assignment σ σ1 ([l0 ↦ (c, [f ↦ l1] (e))] (σ1)) (codom ρ ∪ {ψ}) l0 l1 f c e _ ).
-    destruct H11; eauto.
-    ++ eauto with scoping.
-    ++ eapply_any; eauto with scoping lia wf.
-    ++ eapply scoping_transitivity with _ (codom ρ ∪ {ψ}); eauto with wf.
-       eapply H9; eauto with scoping.
-    ++ split.
-       +++ eapply scoping_transitivity with ([l0 ↦ (c, [f ↦ l1] (e))] (σ1)) (codom ρ ∪ {ψ});
-             update_dom;
-             eauto with wf lia.
-           eapply storeSubset_trans; update_dom; eauto with wf lia.
-           eapply_any; update_dom; eauto with scoping lia.
-       +++ eapply preserving_transitivity; eauto with scoping; update_dom; eauto with wf lia.
-           eapply_any; update_dom; eauto with scoping lia.
+      eapply storeSubset_union.
+      eapply storeSubset_trans; eauto with wf lia.
+      eapply storeSubset_trans; eauto with wf lia.
+      eapply storeSubset_singleton3 ...
+      rewrite dom_app; lia.
+  - (* e = e0.f = e1; e2 *)
+    destruct (getObj σ2 v1) as [[C ω] |] eqn: H__obj.
+    + destruct IHevalP1, IHevalP2 ...
+      destruct IHevalP3; eauto with wf lia.
+      * eapply storeSubset_trans with σ2; eauto with updates ...
+      * eapply scopability_assignment with (f := x) (σ1 := σ) (l' := v2) (L1 := (codom ρ ∪ {ψ})) in H__obj as [ ];
+          try reflexivity; eauto 5 with wf lia scoping.
+        split.
+        -- eapply scoping_transitivity with (σ2 := [v1 ↦ (C, [x ↦ v2] (ω))]σ2) (L2 := codom ρ ∪ {ψ});
+             try eapply H8; eauto 3 with wf lia scoping updates.
+           eapply storeSubset_trans with σ2; eauto with updates wf lia.
+        -- eapply preserving_transitivity; eauto with scoping; update_dom ; eauto with wf lia.
+           eapply_any; update_dom...
+    + destruct IHevalP1, IHevalP2, IHevalP3 ...
+      split .
+      * eapply scoping_transitivity with (σ2 := σ2) (L2 := codom ρ ∪ {ψ}) ...
+      * eapply preserving_transitivity ...
+  - (* el_nil *)
+    split ...
+    intros x; steps.
+    inversion H3; steps.
+  - (* el_cons *)
+    destruct IHevalP, IHevalP0 ...
+    split.
+    + rewrite codom_cons.
+      eapply scoping_union ...
+    + eapply preserving_transitivity_degenerate ...
+  - (* init_cons *)
+    destruct IHevalP; eauto.
+    destruct (getObj σ1 I) as [[C ω] |] eqn:H__obj; [| steps].
+    inversion H__assign; subst.
+    specialize (IHevalP0 L σ0).
+    destruct IHevalP0; eauto with updates wf lia.
+    + eapply scopability_add_env ...
+      eapply H3.
+    + eapply preserving_transitivity; eauto.
+      eapply preserving_transitivity; eauto.
+      unfold scoping_preservation; intros ...
+    + unfold wf; intros; update_dom.
+      getObj_update; flatten; subst; repeat invert_constructor_equalities; subst; eauto.
+      eapply getVal_add in H10; flatten; eauto with wf updates.
 Qed.
